src/num/extra_theories/numpairScript.sml
@@ -6,6 +6,7 @@ open arithmeticTheory BasicProvers TotalDefn
 fun Store_thm(trip as (n,t,tac)) = store_thm trip before export_rewrites [n]
 fun fs ths = FULL_SIMP_TAC (srw_ss() ++ ARITH_ss) ths
 fun simp ths = ASM_SIMP_TAC (srw_ss() ++ ARITH_ss) ths
+val metis_tac = METIS_TAC
 
 val _ = new_theory "numpair"
 
@@ -250,5 +251,32 @@ Proof
   `nsnd (npair n m) <= npair n m` by simp[nsnd_le] >> fs[]
 QED
 
+Theorem npair2_lt_E:
+  npair n n1 < npair n n2 ==> n1 < n2
+Proof
+  simp[npair_def] >> strip_tac >> SPOSE_NOT_THEN ASSUME_TAC
+  >> `n1 >= n2` by simp[]
+  >> `n + n1 >= n + n2` by simp[]
+  >> `n + n2 <= n + n1` by simp[]
+  >> `tri (n + n2) <= tri (n + n1)` by metis_tac[tri_LE]
+  >> `n2 <= n1` by simp[]
+  >> `n2 + tri (n + n2) <= n1 + tri (n + n1)` by simp[]
+  >> fs[]
+QED
+
+
+Theorem npair2_lt_I:
+  n1 < n2 ==> npair n n1 < npair n n2
+Proof
+  rpt strip_tac >> simp[npair_def] >>
+  `n + n1 < n + n2` by simp[] >>
+  `tri (n + n1) < tri (n + n2)` by simp[tri_LT] >> simp[]
+QED
+
+Theorem npair2_lt[simp]:
+  npair n n1 < npair n n2 <=> n1 < n2
+Proof
+  metis_tac[npair2_lt_E, npair2_lt_I]
+QED
 
 val _ = export_theory()
